seq fixed

specs/Spec.Chacha20.fst
@@ -15,11 +15,11 @@ let noncelen = 12 (* in bytes *)
 type key = lbytes keylen
 type block = lbytes blocklen
 type nonce = lbytes noncelen
-type counter = size_t
+type counter = size_nat
 
 // Internally, blocks are represented as 16 x 4-byte integers
 type state = m:intseq U32 16
-type idx = n:size_t{n < 16}
+type idx = n:size_nat{n < 16}
 type shuffle = state -> Tot state
 
 // Using @ as a functional substitute for ;
