specs/lib/Spec.Lib.IntBuf.fsti
@@ -6,10 +6,11 @@ open Spec.Lib.IntTypes
 
 module LSeq = Spec.Lib.IntSeq
 
-
+inline_for_extraction
+let v = size_v 
 inline_for_extraction val lbuffer: a:Type0 -> len:size_t -> Type0
-inline_for_extraction val sub: #a:Type0 -> #len:size_t -> b:lbuffer a len -> start:size_t -> n:size_t{start + n <= len} -> Tot (lbuffer a n)
- let slice #a #len (b:lbuffer a len) (start:size_t) (fin:size_t{fin <= len /\ start <= fin}) = sub #a #len b start (fin - start)
+inline_for_extraction val sub: #a:Type0 -> #len:size_t -> b:lbuffer a len -> start:size_t -> n:size_t{v start + v n <= v len} -> Tot (lbuffer a n)
+ let slice #a #len (b:lbuffer a len) (start:size_t) (fin:size_t{v fin <= v len /\ v start <= v fin}) = sub #a #len b start (sub_mod #SIZE fin start)
 noeq type bufitem = | BufItem: #a:Type0 -> #len:size_t -> buf:lbuffer a len -> bufitem
 
 
@@ -47,9 +48,9 @@ inline_for_extraction val create: #a:Type0 -> len:size_t -> init:a -> StackInlin
 					    modifies1 r h0 h1 /\ 
 					    as_lseq #a #len r h1 == LSeq.create #a len init))
 		      
-inline_for_extraction val createL: #a:Type0 -> init:list a{List.Tot.length init <= max_size_t} -> StackInline (lbuffer a (List.Tot.length init))
+inline_for_extraction val createL: #a:Type0 -> init:list a{List.Tot.length init <= max_size_t} -> StackInline (lbuffer a (size (List.Tot.length init)))
 		      (requires (fun h0 -> True))
-		      (ensures (fun h0 r h1 -> preserves_live h0 h1 /\ creates1 r h0 h1 /\ modifies1 r h0 h1 /\ as_lseq #a #(List.Tot.length init) r h1 == LSeq.createL #a init))
+		      (ensures (fun h0 r h1 -> preserves_live h0 h1 /\ creates1 r h0 h1 /\ modifies1 r h0 h1 /\ as_lseq #a #(size (List.Tot.length init)) r h1 == LSeq.createL #a init))
 
 inline_for_extraction val alloc: #a:Type0 -> #b:Type0 -> len:size_t -> init:a -> 
 		 reads:list bufitem ->
@@ -67,30 +68,30 @@ inline_for_extraction val alloc: #a:Type0 -> #b:Type0 -> len:size_t -> init:a ->
 					    spec h0 r h1))
 
 
-inline_for_extraction val index: #a:Type0 -> #len:size_t -> b:lbuffer a len -> i:size_t{i < len} -> Stack a 
+inline_for_extraction val index: #a:Type0 -> #len:size_t -> b:lbuffer a len -> i:size_t{v i < v len} -> Stack a 
 		      (requires (fun h0 -> live h0 b))
 		      (ensures (fun h0 r h1 -> h0 == h1 /\ r == LSeq.index #a #len (as_lseq #a #len b h0) i)) 
 
-inline_for_extraction val upd: #a:Type0 -> #len:size_t -> b:lbuffer a len -> i:size_t{i < len} -> v:a -> Stack unit 
-		      (requires (fun h0 -> live h0 b /\ len > 0))
-		      (ensures (fun h0 r h1 -> preserves_live h0 h1 /\ modifies1 b h0 h1 /\ as_lseq #a #len b h1 == LSeq.upd #a #len (as_lseq #a #len b h0) i v))
+inline_for_extraction val upd: #a:Type0 -> #len:size_t -> b:lbuffer a len -> i:size_t{v i < v len} -> x:a -> Stack unit 
+		      (requires (fun h0 -> live h0 b /\ v len > 0))
+		      (ensures (fun h0 r h1 -> preserves_live h0 h1 /\ modifies1 b h0 h1 /\ as_lseq #a #len b h1 == LSeq.upd #a #len (as_lseq #a #len b h0) i x))
 
 inline_for_extraction let op_Array_Assignment = upd
 inline_for_extraction let op_Array_Access = index
 
-noextract
- val map: #a:Type -> #len:size_t -> f:(a -> Tot a) -> b:lbuffer a len -> Stack unit 
+val map: #a:Type -> #len:size_t -> f:(a -> Tot a) -> b:lbuffer a len -> Stack unit 
 		      (requires (fun h0 -> live h0 b))
 		      (ensures (fun h0 _ h1 -> preserves_live h0 h1 /\ modifies1 b h0 h1 /\ as_lseq #a #len b h1 == LSeq.map #a #a #len f (as_lseq #a #len b h0)))
 
-noextract
- val map2: #a1:Type -> #a2:Type -> #len:size_t -> f:(a1 -> a2 -> Tot a1) -> b1:lbuffer a1 len -> b2:lbuffer a2 len -> Stack unit 
+inline_for_extraction
+val map2: #a1:Type -> #a2:Type -> #len:size_t -> f:(a1 -> a2 -> Tot a1) -> b1:lbuffer a1 len -> b2:lbuffer a2 len -> Stack unit 
 		      (requires (fun h0 -> live h0 b1 /\ live h0 b2))
 		      (ensures (fun h0 _ h1 -> preserves_live h0 h1 /\ modifies1 b1 h0 h1 /\ as_lseq #a1 #len b1 h1 == LSeq.map2 #a1 #a2 #a1 #len f (as_lseq #a1 #len b1 h0) (as_lseq #a2 #len b2 h0)))
 
-noextract val blit: #a:Type -> #len:size_t -> i:lbuffer a len -> start1:size_t -> 
+val blit: #a:Type -> #len:size_t -> i:lbuffer a len -> start1:size_t -> 
           o:lbuffer a len -> start2:size_t -> 
-	  num:size_t{start1 + num <= len /\ start2 + num <= len} -> Stack unit 
+	  num:size_t{v start1 + v num <=  v len /\ v start2 + v num <= v len} -> 
+	  Stack unit 
  		  (requires (fun h0 -> live h0 i /\ live h0 o ))
   		  (ensures (fun h0 _ h1 -> preserves_live h0 h1 /\ 
 		  			modifies1 o h0 h1 /\ 
@@ -99,14 +100,15 @@ noextract val blit: #a:Type -> #len:size_t -> i:lbuffer a len -> start1:size_t -
 						start1 num
 						(LSeq.sub (as_lseq i h0) start2 num)))
 
-noextract val copy: #a:Type -> #len:size_t -> i:lbuffer a len -> o:lbuffer a len -> Stack unit 
+inline_for_extraction
+val copy: #a:Type -> #len:size_t -> i:lbuffer a len -> o:lbuffer a len -> Stack unit 
  		  (requires (fun h0 -> live h0 i /\ live h0 o ))
   		  (ensures (fun h0 _ h1 -> preserves_live h0 h1 /\ 
 		  			modifies1 o h0 h1 /\ 
 					as_lseq o h1 == as_lseq i h0))
 
 
-noextract val repeat: #a:Type -> #b:Type -> #lift:(mem -> b -> GTot (option a)) -> 
+val repeat: #a:Type -> #b:Type -> #lift:(mem -> b -> GTot (option a)) -> 
 	    n:size_t -> spec:(a -> Tot a) -> 
 	    impl:(x:b -> Stack unit (requires (fun h0 -> Some? (lift h0 x))) (ensures (fun h0 _ h1 -> Some? (lift h0 x) /\ Some? (lift h1 x) /\ Some?.v (lift h1 x) == spec (Some?.v (lift h0 x))))) ->
 	    input:b ->
@@ -116,9 +118,9 @@ noextract val repeat: #a:Type -> #b:Type -> #lift:(mem -> b -> GTot (option a)) 
 				  Some?.v (lift h1 input) ==  LSeq.repeat n spec (Some?.v (lift h0 input))))
 
 
-noextract val repeat_range: #a:Type -> #b:Type -> #lift:(mem -> b -> GTot (option a)) -> 
-	    start:size_t -> fin:size_t{start <= fin} -> spec:(i:size_t{start <= i /\ i < fin} -> a -> Tot a) -> 
-	    impl:(i:size_t{start <= i /\ i < fin} -> x:b -> Stack unit 
+val repeat_range: #a:Type -> #b:Type -> #lift:(mem -> b -> GTot (option a)) -> 
+	    start:size_t -> fin:size_t{v start <= v fin} -> spec:(i:size_t{v start <= v i /\ v i < v fin} -> a -> Tot a) -> 
+	    impl:(i:size_t{v start <= v i /\ v i < v fin} -> x:b -> Stack unit 
 				   (requires (fun h0 -> Some? (lift h0 x))) 
 				   (ensures (fun h0 _ h1 -> Some? (lift h0 x) /\ Some? (lift h1 x) /\ 
 							 Some?.v (lift h1 x) == spec i (Some?.v (lift h0 x))))) ->
@@ -128,9 +130,9 @@ noextract val repeat_range: #a:Type -> #b:Type -> #lift:(mem -> b -> GTot (optio
 	    (ensures (fun h0 _ h1 -> Some? (lift h0 input) /\ Some? (lift h1 input) /\
 				  Some?.v (lift h1 input) ==  LSeq.repeat_range start fin spec (Some?.v (lift h0 input))))
 
-noextract val repeati: #a:Type -> #b:Type -> #lift:(mem -> b -> GTot (option a)) -> 
-	    n:size_t -> spec:(i:size_t{i < n} -> a -> Tot a) -> 
-	    impl:(i:size_t{i < n} -> x:b -> Stack unit 
+val repeati: #a:Type -> #b:Type -> #lift:(mem -> b -> GTot (option a)) -> 
+	    n:size_t -> spec:(i:size_t{v i < v n} -> a -> Tot a) -> 
+	    impl:(i:size_t{v i < v n} -> x:b -> Stack unit 
 				   (requires (fun h0 -> Some? (lift h0 x))) 
 				   (ensures (fun h0 _ h1 -> Some? (lift h0 x) /\ Some? (lift h1 x) /\ 
 							 Some?.v (lift h1 x) == spec i (Some?.v (lift h0 x))))) ->
@@ -139,8 +141,9 @@ noextract val repeati: #a:Type -> #b:Type -> #lift:(mem -> b -> GTot (option a))
 	    (requires (fun h0 -> Some? (lift h0 input)))
 	    (ensures (fun h0 _ h1 -> Some? (lift h0 input) /\ Some? (lift h1 input) /\
 				  Some?.v (lift h1 input) ==  LSeq.repeati n spec (Some?.v (lift h0 input))))
-
-noextract val iter: #a:Type -> #len:size_t -> n:size_t -> spec:(LSeq.lseq a len -> Tot (LSeq.lseq a len)) -> 
+				  
+inline_for_extraction
+val iter: #a:Type -> #len:size_t -> n:size_t -> spec:(LSeq.lseq a len -> Tot (LSeq.lseq a len)) -> 
          impl:(x:lbuffer a len -> Stack unit 
 			(requires (fun h0 -> live h0 x))
 			(ensures (fun h0 _ h1 -> preserves_live h0 h1 /\ 
@@ -152,8 +155,8 @@ noextract val iter: #a:Type -> #len:size_t -> n:size_t -> spec:(LSeq.lseq a len 
 	    (ensures (fun h0 _ h1 -> preserves_live h0 h1 /\ modifies1 input h0 h1 /\
 				  as_lseq #a #len input h1 ==  LSeq.repeat n spec (as_lseq #a #len input h0)))
 
-noextract val iteri: #a:Type -> #len:size_t -> n:size_t -> spec:(i:size_t{i < n}  -> LSeq.lseq a len -> Tot (LSeq.lseq a len)) -> 
-         impl:(i:size_t{i < n}  -> x:lbuffer a len -> Stack unit 
+val iteri: #a:Type -> #len:size_t -> n:size_t -> spec:(i:size_t{v i < v n}  -> LSeq.lseq a len -> Tot (LSeq.lseq a len)) -> 
+         impl:(i:size_t{v i < v n}  -> x:lbuffer a len -> Stack unit 
 			(requires (fun h0 -> live h0 x))
 			(ensures (fun h0 _ h1 -> preserves_live h0 h1 /\ 
 				              modifies1 x h0 h1 /\
@@ -164,9 +167,9 @@ noextract val iteri: #a:Type -> #len:size_t -> n:size_t -> spec:(i:size_t{i < n}
 	    (ensures (fun h0 _ h1 -> preserves_live h0 h1 /\ modifies1 input h0 h1 /\
 				  as_lseq #a #len input h1 ==  LSeq.repeati n spec (as_lseq #a #len input h0)))
 
-noextract val iter_range: #a:Type -> #len:size_t -> start:size_t -> fin:size_t{start <= fin} ->
-         spec:(i:size_t{start <= i /\ i < fin}  -> LSeq.lseq a len -> Tot (LSeq.lseq a len)) -> 
-         impl:(i:size_t{start <= i /\ i < fin}  -> x:lbuffer a len -> Stack unit 
+val iter_range: #a:Type -> #len:size_t -> start:size_t -> fin:size_t{v start <= v fin} ->
+         spec:(i:size_t{v start <= v i /\ v i < v fin}  -> LSeq.lseq a len -> Tot (LSeq.lseq a len)) -> 
+         impl:(i:size_t{v start <= v i /\ v i < v fin}  -> x:lbuffer a len -> Stack unit 
 			(requires (fun h0 -> live h0 x))
 			(ensures (fun h0 _ h1 -> preserves_live h0 h1 /\ 
 				              modifies1 x h0 h1 /\
@@ -178,10 +181,10 @@ noextract val iter_range: #a:Type -> #len:size_t -> start:size_t -> fin:size_t{s
 				  as_lseq #a #len input h1 ==  LSeq.repeat_range start fin spec (as_lseq #a #len input h0)))
 
 
-noextract val uints_from_bytes_le: 
-  #t:inttype -> #len:size_t{len `op_Multiply` numbytes t <= max_size_t} -> 
+val uints_from_bytes_le: 
+  #t:inttype -> #len:size_t{v len `op_Multiply` numbytes t <= max_size_t} -> 
   o:lbuffer (uint_t t) len ->
-  i:lbuffer uint8 (len `op_Multiply` numbytes t) -> 
+  i:lbuffer uint8 (mul_mod #SIZE len (size (numbytes t))) -> 
   Stack unit 
 	(requires (fun h0 -> live h0 o /\ live h0 i))
 	(ensures (fun h0 _ h1 -> preserves_live h0 h1 /\
@@ -190,10 +193,10 @@ noextract val uints_from_bytes_le:
 			      (LSeq.uints_from_bytes_le #t #len (as_lseq i h0) )))
 
 
-noextract val uint32s_from_bytes_le: 
-  #len:size_t{len `op_Multiply` 4 <= max_size_t} -> 
+val uint32s_from_bytes_le: 
+  #len:size_t{v len `op_Multiply` 4 <= max_size_t} -> 
   o:lbuffer uint32 len ->
-  i:lbuffer uint8 (len `op_Multiply` 4) -> 
+  i:lbuffer uint8 (mul_mod #SIZE len (size 4)) -> 
   Stack unit 
 	(requires (fun h0 -> live h0 o /\ live h0 i))
 	(ensures (fun h0 _ h1 -> preserves_live h0 h1 /\
@@ -201,9 +204,9 @@ noextract val uint32s_from_bytes_le:
 			      as_lseq o h1 == 
 			      (LSeq.uints_from_bytes_le #U32 #len (as_lseq i h0) )))
 
-noextract val uint32s_to_bytes_le: 
-  #len:size_t{len `op_Multiply` 4 <= max_size_t} -> 
-  o:lbuffer uint8 (len `op_Multiply` 4) -> 
+val uint32s_to_bytes_le: 
+  #len:size_t{v len `op_Multiply` 4 <= max_size_t} -> 
+  o:lbuffer uint8 (mul_mod #SIZE len (size 4)) -> 
   i:lbuffer uint32 len ->
   Stack unit 
 	(requires (fun h0 -> live h0 o /\ live h0 i))
