specs/lib/Spec.Lib.Stateful.fsti
@@ -6,18 +6,18 @@ noeq type state_def =
   | StateDef: state: Type0 ->
 	      key:Type0 ->
 	      value:(key->Type0) ->
-	      length:(key->size_t) ->
+	      length:(key->size_nat) ->
 	      create:(unit -> state) ->
 	      get:(state -> k:key -> lseq (value k) (length k)) ->
 	      put:(state -> k:key -> lseq (value k) (length k) -> state) ->
 	      state_def
 
 unfold
-let state_index (d:state_def) (k:d.key) = s:size_t{s < d.length k}
+let state_index (d:state_def) (k:d.key) = s:size_nat{s < d.length k}
 unfold
 let state_seq (d:state_def) (k:d.key) : Type0 = lseq (d.value k) (d.length k)
 unfold
-let state_slice (d:state_def) (k:d.key) (min:size_t) (max:size_t{min <= max}) : Type0 = lseq (d.value k) (max - min)
+let state_slice (d:state_def) (k:d.key) (min:size_nat) (max:size_nat{min <= max}) : Type0 = lseq (d.value k) (max - min)
 
 
 val stateful (d:state_def) (a:Type0) : Type0
@@ -31,11 +31,11 @@ val bind: #a:Type0 -> #b:Type0 -> #d:state_def -> f:stateful d a -> g:(a -> stat
 
 (* Convenience functions, can be implemented using read/write and repeat_range *)
 
-val repeat_stateful: #d:state_def -> n:size_t -> f:stateful d unit -> stateful d unit
-val repeat_range_stateful: #d:state_def -> min:size_t -> max:size_t{min <= max} -> f:(i:size_t{i >= min /\ i < max} -> stateful d unit) -> stateful d unit
+val repeat_stateful: #d:state_def -> n:size_nat -> f:stateful d unit -> stateful d unit
+val repeat_range_stateful: #d:state_def -> min:size_nat -> max:size_nat{min <= max} -> f:(i:size_nat{i >= min /\ i < max} -> stateful d unit) -> stateful d unit
 val copy: #d:state_def -> k1:d.key -> k2:d.key{d.value k1 == d.value k2 /\ d.length k1 == d.length k2} -> stateful d unit
 val in_place_map2: #d:state_def -> k1:d.key -> k2:d.key{d.value k1 == d.value k2 /\ d.length k1 == d.length k2} -> f:(d.value k1 -> d.value k2 -> d.value k2) -> stateful d unit
-val import: #a:Type0 -> #len:size_t -> #d:state_def -> lseq a len -> k:d.key -> f:(lseq a len -> state_seq d k) -> stateful d unit
-val import_slice: #a:Type0 -> #len:size_t -> #d:state_def -> lseq a len -> k:d.key -> min:size_t -> max:size_t{min <= max /\ max <= d.length k} -> f:(lseq a len -> state_slice d k min max) -> stateful d unit
+val import: #a:Type0 -> #len:size_nat -> #d:state_def -> lseq a len -> k:d.key -> f:(lseq a len -> state_seq d k) -> stateful d unit
+val import_slice: #a:Type0 -> #len:size_nat -> #d:state_def -> lseq a len -> k:d.key -> min:size_nat -> max:size_nat{min <= max /\ max <= d.length k} -> f:(lseq a len -> state_slice d k min max) -> stateful d unit
 
-val export: #a:Type0 -> #len:size_t -> #d:state_def -> k:d.key -> f:(state_seq d k -> lseq a len) -> stateful d (lseq a len)
+val export: #a:Type0 -> #len:size_nat -> #d:state_def -> k:d.key -> f:(state_seq d k -> lseq a len) -> stateful d (lseq a len)
